avltree/AvlBase.lean
@@ -1,0 +1,3 @@
+import avltree.TreeBase
+
+open TreeBase_n
